Temporary work.

src/coq/procedure/Procedure.v
@@ -16,38 +16,42 @@ Import ImpModel .
     | aExp : AExp -> AExp .
 
 
-Notation "A + B" := (aExpPlus A B) .
-
-
+  Notation "A + B" := (aExpPlus A B) .
+  Notation "A / B" := (aExpDiv A B) .
+  Notation "A * B" := (aExpMult A B) .
+  Notation "$ A" := (aExpId A) (at level 40).
 
   (* Boolean expressions *)
   Inductive BExp :=
     | bExpBool : SymBool -> BExp
     | bExpNeg : BExp -> BExp 
     | bExpLeq : AExp -> AExp -> BExp 
+    | bExpLe  : AExp -> AExp -> BExp 
+    | bExpEq  : AExp -> AExp -> BExp 
     | bExpAnd : BExp -> BExp -> BExp
     | bExp : BExp -> BExp .
 
-
-  Scheme Equality for BExp .
-  
+  Notation "! B" := (bExpNeg B) (at level 75) .
+  Notation "A && B" := (bExpAnd A B) .
+  Notation "A <= B" := (bExpLeq A B) .
+  Notation "A = B" := (bExpEq A B) .
   
   (* Stmts *)
   Inductive Stmt :=
     | stmtAssign : string -> AExp -> Stmt
     | stmtIfElse : BExp -> Stmt -> Stmt -> Stmt 
     | stmtWhile : BExp -> Stmt -> Stmt 
-    | stmtList : Stmt -> Stmt -> Stmt 
+    | stmtList : Stmt -> Stmt -> Stmt
     | stmtSkip : Stmt .
-
-Scheme Equality for Stmt.
-  Print Stmt_beq.
-
+  
+  Notation "S1 ; S2" := (stmtList S1 S2) (at level 89, left associativity).
+(*  Notation "A := B" := (stmtAssign A B) (at level 88, right associativity). *)
+  
   (* K sequence *)
   Inductive KSequence :=
     | kra : Stmt -> KSequence -> KSequence 
     | kdot : KSequence .
-  Notation "K ~> K'" := (kra K K') (at level 99).
+  Notation "K ~> K'" := (kra K K') (at level 91, left associativity).
 
   (* Configuration *)
   Inductive Cfg : Type := cfg : KSequence -> State -> Cfg .
@@ -55,7 +59,14 @@ Scheme Equality for Stmt.
   (* Finally, the terms *)
   Definition Term : Type := Cfg .
 
+  Scheme Equality for KSequence.
+  Scheme Equality for SymInt.
+  Scheme Equality for SymBool.
 
+  
+  Definition Term_beq (T1 T2 : Term) :=
+    match T1, T2 with
+      | cfg KS1 S1, cfg KS2 S2 => andb (KSequence_beq KS1 KS2) (State_beq S1 S2)    end.   
 
 
 
@@ -80,90 +91,194 @@ Inductive Formula : Type :=
   | symF : SymBool -> Formula 
 .
 
-(* Rules = Reachability Logic formulas *)
+
 Inductive Rule : Type := rule : Formula -> Formula -> Rule .
 Notation "L => R" := (rule L R) (at level 100) .
 
 
-
-(* TODO: either implement this correctly or search for a different solution *)
-Fixpoint beqFormula (F1 : Formula) (F2 : Formula) : bool :=
+Fixpoint Formula_beq (F1 : Formula) (F2 : Formula) : bool :=
   match F1, F2 with
-    | bp pi, bp pi' => true (* TODO: fix this *)
+    | bp pi, bp pi' => (Term_beq pi pi')
     | T, T => true
-    | notF F11, notF F22 => beqFormula F11 F22
+    | notF F11, notF F22 => Formula_beq F11 F22
     | andF F11 F12, andF F21 F22
-      => andb (beqFormula F11 F21) (beqFormula F21 F22)
-    | orF F11 F12, andF F21 F22
-      => orb (beqFormula F11 F21) (beqFormula F21 F22)
-    | impliesF F11 F12, andF F21 F22
-      => implb (beqFormula F11 F21) (beqFormula F21 F22)
-    | existsF V1 F11, existsF V2 F22
-      => beqFormula F11 F22 (* TODO: fix this *)
-    | symF _, symF _ => true (* TODO: fix this *)
+      => andb (Formula_beq F11 F21) (Formula_beq F12 F22)
+    | orF F11 F12, orF F21 F22
+      => orb (Formula_beq F11 F21) (Formula_beq F12 F22)
+    | impliesF F11 F12, impliesF F21 F22
+      => andb (Formula_beq F11 F21) (Formula_beq F12 F22)
+    | symF F1, symF F2 => SymBool_beq F1 F2
     | _, _ => false 
   end.
 
-(* TODO: why not using strings as keys for maps ? *)
-Fixpoint beqRule (R1 : Rule) (R2 : Rule) : bool :=
+Fixpoint Rule_beq (R1 : Rule) (R2 : Rule) : bool :=
   match R1, R2 with
     | (phi1 => phi1'), (phi2 => phi2') =>
-      andb (beqFormula phi1 phi2) (beqFormula phi1' phi2')
+      andb (Formula_beq phi1 phi2) (Formula_beq phi1' phi2')
   end.
 
 Fixpoint beqListRule (L1 : list Rule) (L2 : list Rule) : bool :=
   match L1, L2 with
     | nil, nil => true
-    | r1 :: tl1, r2 :: tl2 => andb (beqRule r1 r2) (beqListRule tl1 tl2)
+    | r1 :: tl1, r2 :: tl2 => andb (Rule_beq r1 r2) (beqListRule tl1 tl2)
     | _, _ => false
   end.
 
+
+
+
+
+
+
+
+
+
+
+
+
+
+
+
+
+
+
+(* Semantics *)
+
+  Fixpoint evalAexp (s : State) (e : AExp) :=
+    match e with
+      | aExpSymInt x => Some x
+      | aExpId x => lookup x s
+      | aExpDiv e1 e2 => match evalAexp s e1, evalAexp s e2 with
+                           | Some v1, Some v2 => Some (symDiv v1 v2) 
+                           | _, _ => None                           
+                         end
+      | aExpMult e1 e2 => match evalAexp s e1, evalAexp s e2 with
+                            | Some v1, Some v2 => Some (symMult v1 v2)
+                            | _, _ => None                           
+                          end
+      | aExpPlus e1 e2 => match evalAexp s e1, evalAexp s e2 with
+                            | Some v1, Some v2 => Some (symPlus v1 v2)
+                            | _, _ => None                           
+                          end
+      | aExp e => evalAexp s e
+    end.
+
+  Fixpoint evalBexp (s : State) (be : BExp) :=
+    match be with
+      | bExpBool b => Some b
+      | bExpNeg b => match evalBexp s b with
+                       | Some v => Some (symNeg v)
+                       | _ => None
+                     end
+      | bExpLeq e1 e2 => match evalAexp s e1, evalAexp s e2 with
+                           | Some v1, Some v2 => Some (symLeqInt v1 v2)
+                           | _, _ => None
+                         end
+      | bExpLe e1 e2 => match evalAexp s e1, evalAexp s e2 with
+                           | Some v1, Some v2 => Some (symLeInt v1 v2)
+                           | _, _ => None
+                         end
+      | bExpEq e1 e2 => match evalAexp s e1, evalAexp s e2 with
+                           | Some v1, Some v2 => Some (symEqInt v1 v2)
+                           | _, _ => None
+                         end
+      | bExpAnd b1 b2 => match evalBexp s b1, evalBexp s b2 with
+                           | Some v1, Some v2 => Some (symAnd v1 v2)
+                           | _, _ => None
+                         end
+      | bExp b => evalBexp s b
+    end.
+
+  
+Inductive Sem : Rule -> Prop :=
+  | stepAssign : forall Env Env' X E V P K,
+                   evalAexp Env E = Some V -> update X V Env = Some Env' ->
+                   Sem (rule
+                        (andF (bp (cfg (kra (stmtAssign X E) K) Env)) P)
+                        (andF (bp (cfg (kra stmtSkip K) Env')) P))
+  | stepIfThen : forall St1 St2 Env B K P C,
+                   evalBexp Env B = Some C ->
+                   Sem (rule
+                        (andF (bp (cfg (kra (stmtIfElse B St1 St2) K) Env)) (symF P))
+                           (andF (bp (cfg (kra St1 K) Env))
+                                 (symF (symAnd C P)))
+                       )
+  | stepIfElse : forall St1 St2 Env B K P C,
+                   evalBexp Env B = Some C ->
+                   Sem (rule
+                        (andF (bp (cfg (kra (stmtIfElse B St1 St2) K) Env)) (symF P))
+                           (andF (bp (cfg (kra St2 K) Env))
+                                 (symF (symAnd (symNeg C) P)))
+                       )
+  | stepWhile : forall St Env B K P,
+                  Sem (rule
+                       (andF (bp (cfg (kra (stmtWhile B St) K) Env)) P)
+                       (andF (bp (cfg (kra (stmtIfElse B (stmtList St (stmtWhile B St)) stmtSkip) K) Env)) P))
+  | stepList : forall St1 St2 Env K P,
+                 Sem (rule
+                      (andF (bp (cfg (kra (stmtList St1 St2) K) Env)) P)
+                      (andF (bp (cfg (kra St1 (kra St2 K)) Env)) P))
+  | stepSkip : forall Env K P,
+                 Sem (rule
+                      (andF (bp (cfg (kra stmtSkip K) Env)) P)
+                      (andF (bp (cfg K Env)) P)) .
+
+
+
+
+
+
+
+
+
+
+
+
+
+
+
+
 Fixpoint bGetFromMap (M : Map Formula bool) (phi : Formula) : bool :=
-  match (Map.get Formula bool M phi beqFormula) with
+  match (Map.get Formula bool M phi Formula_beq) with
     | None => false
     | Some v => v
   end.
 
 
-
-Fixpoint delta (r : Rule) (R : list Rule)
+Fixpoint get_two (r : Rule) (R : list Rule)
          (M : Map Rule (Map (list Rule) (list Rule))) :=
-  match Map.get Rule (Map (list Rule) (list Rule)) M r beqRule with
+  match Map.get Rule (Map (list Rule) (list Rule)) M r Rule_beq with
     | Some v => match Map.get (list Rule) (list Rule) v R beqListRule with
                   | Some l => l
                   | None => nil
                 end
     | None => nil
   end.
-
-
-
-Eval compute in ((1,2) :: nil) ++ ((2,3) ::nil).
-
+                                                                
+                                                   
 Fixpoint prove (n : nat) (G0 G S : list Rule)
-               (Valid : Map Formula bool)
-               (DerivableS : Map Formula bool) (* TODO : S parameter *)
-               (DeltaS : Map Rule (Map (list Rule) (list Rule))) (* TODO : S parameter *)
-               (DeltaCirc : Map Rule (Map (list Rule) (list Rule))) (* TODO : Circ parameter *)
-               (ChooseCirc : Map Formula Rule) :=
+               (Valid : Map Formula bool) 
+               (Derivable : Map Formula bool) (* TODO : S parameter *)
+               (Delta : Map Rule (Map (list Rule) (list Rule)))
+               (ChooseCirc : Map Formula Rule) (* consistency? *) :=
   match n with
     | 0 => false
     | S m => match G with
                | nil => true
                | (phi => phi') :: Rest =>
                  if (bGetFromMap Valid (impliesF phi phi'))
-                 then prove m G0 Rest S Valid DerivableS DeltaS DeltaCirc ChooseCirc
+                 then prove m G0 Rest S Valid Derivable Delta ChooseCirc
                  else
-                   match Map.get Formula Rule ChooseCirc phi beqFormula  with
+                   match Map.get Formula Rule ChooseCirc phi Formula_beq  with
                      | Some circ => prove m G0
-                                          ((delta (phi => phi') (circ :: nil)
-                                                  DeltaCirc) ++ Rest)
-                                          S Valid DerivableS DeltaS DeltaCirc ChooseCirc
+                                          ((get_two (phi => phi') (circ :: nil)
+                                                  Delta) ++ Rest)  (* rule, Sem -> Derivatives
+                                          S Valid Derivable Delta ChooseCirc
                                             
-                     | None => if (bGetFromMap DerivableS phi)
+                     | None => if (bGetFromMap Derivable phi)
                                then prove m G0
-                                          ((delta (phi => phi') S DeltaS) ++ Rest)
-                                          S Valid DerivableS DeltaS DeltaCirc ChooseCirc
+                                          ((delta (phi => phi') S Delta) ++ Rest)
+                                          S Valid Derivable Delta ChooseCirc
                                else false
                    end
              end
@@ -173,29 +288,208 @@ Extraction prove .
 
 
 (* Testing *)
+Open Scope string_scope.
+Definition phi :=
+  (andF
+     (bp 
+        (cfg (kra (stmtWhile (bExpLe (aExpId "i") (aExpId "n")) (stmtAssign "i" ($ "i" + aExpSymInt (symZ 1)))) kdot)
+             (("i", symInt "I")::("n", symInt "N")::nil)))
+     (symF (symLeqInt (symInt "I") (symInt "N")))).
+
+Definition phi' :=
+  (andF
+     (bp (cfg kdot
+             (("i", (symPlus (symInt "I") (symZ 1)))::("n", symInt "N")::nil)))
+     (symF (symLeqInt (symInt "N") (symInt "I")))).
+
+
+Definition phi1 :=
+  (andF
+     (bp 
+        (cfg (kra
+                (stmtIfElse (bExpLe (aExpId "i") (aExpId "n"))
+                            (stmtList
+                               (stmtAssign "i" ($ "i" + aExpSymInt (symZ 1)))
+                               (stmtWhile (bExpLe (aExpId "i") (aExpId "n")) (stmtAssign "i" ($ "i" + aExpSymInt (symZ 1))))
+                            )
+                            stmtSkip
+                )
+                                 kdot)
+             (("i", symInt "I")::("n", symInt "N")::nil)))
+     (symF (symLeqInt (symInt "I") (symInt "N")))).
+
+
+Check stepIfElse.
+
+Definition phi21 :=
+     (andF
+        (bp 
+           (cfg (kra
+                   (stmtList
+                      (stmtAssign "i" ($ "i" + aExpSymInt (symZ 1)))
+                      (stmtWhile (bExpLe (aExpId "i") (aExpId "n")) (stmtAssign "i" ($ "i" + aExpSymInt (symZ 1))))
+                   )
+                   kdot)
+                (("i", symInt "I")::("n", symInt "N")::nil)))
+        (symF (symAnd
+                 (symLeInt (symInt "I") (symInt "N"))
+                 (symLeqInt (symInt "I") (symInt "N")))
+        ))
+.
+
+Definition phi22 :=
+     (andF
+        (bp 
+           (cfg (kra stmtSkip kdot)
+                (("i", symInt "I")::("n", symInt "N")::nil)))
+        (symF (symAnd
+                 (symNeg (symLeInt (symInt "I") (symInt "N")))
+                 (symLeqInt (symInt "I") (symInt "N")))
+        ))
+   .
+
+Check stepList.
+   
+Definition phi3 := 
+     (andF
+        (bp 
+           (cfg (kra
+                   
+                   (stmtAssign "i" ($ "i" + aExpSymInt (symZ 1)))
+                   (kra
+                      (stmtWhile (bExpLe (aExpId "i") (aExpId "n")) (stmtAssign "i" ($ "i" + aExpSymInt (symZ 1))))
+                      kdot)
+                   )
+                (("i", symInt "I")::("n", symInt "N")::nil)))
+        (symF (symAnd
+                 (symLeInt (symInt "I") (symInt "N"))
+                 (symLeqInt (symInt "I") (symInt "N")))
+        ))
+.
+
+
+Check stepAssign.
+
+Definition phi4 :=
+     (andF
+        (bp 
+           (cfg (kra
+                   stmtSkip
+                   (kra
+                      (stmtWhile (bExpLe (aExpId "i") (aExpId "n")) (stmtAssign "i" ($ "i" + aExpSymInt (symZ 1))))
+                      kdot)
+                )
+                (("i", (symPlus (symInt "I") (symZ 1)))::("n", symInt "N")::nil)))
+        (symF (symAnd
+                 (symLeInt (symInt "I") (symInt "N"))
+                 (symLeqInt (symInt "I") (symInt "N")))
+        )).
+
+
+Definition phi5 := 
+     (andF
+        (bp 
+           (cfg
+              (kra
+                 (stmtWhile (bExpLe (aExpId "i") (aExpId "n")) (stmtAssign "i" ($ "i" + aExpSymInt (symZ 1))))
+                 kdot)
+                
+              (("i", (symPlus (symInt "I") (symZ 1)))::("n", symInt "N")::nil)))
+        (symF (symAnd
+                 (symLeInt (symInt "I") (symInt "N"))
+                 (symLeqInt (symInt "I") (symInt "N")))
+        )).
+
+
+Lemma tr1 : exists phi', Sem (phi => phi') .
+  exists phi1.
+  apply stepWhile.
+Qed.
+
+
+Lemma tr21 : exists phi', Sem (phi1 => phi').
+  exists phi21.
+  apply stepIfThen.
+  simpl. trivial.
+Qed.
+
+Lemma tr22 : exists phi', Sem (phi1 => phi').
+  exists phi22.
+  apply stepIfElse.
+  simpl. trivial.
+Qed.
+
+Lemma tr3 : exists phi', Sem (phi21 => phi') .
+  exists phi3.
+  apply stepList.
+Qed.
+
+Lemma tr4 : exists phi', Sem (phi3 => phi') .
+  exists phi4.
+  eapply stepAssign; simpl; trivial.
+Qed.
+
+Lemma tr5 : exists phi', Sem (phi4 => phi') .
+  exists phi5.
+  eapply stepSkip.
+Qed.
+
 
 (*
-Definition DeltaS : Map Formula Formula := nil .
-Definition DeltaCirc : Map Formula Formula := nil .
-Definition Valid : Map Formula bool := nil .
-Definition Derivable : Map Formula bool := nil .
+               (Valid : Map Formula bool)
+               (Derivable : Map Formula bool)
+               (Delta : Map Rule (Map (list Rule) (list Rule)))
+               (ChooseCirc : Map Formula Rule) :=
+
+ *)
+Definition Derivable1 : Map Formula bool := (phi, true)
+                       :: (phi1, true)
+                       :: (phi21, true)
+                       :: (phi3, true)
+                       :: (phi4, true)
+                       :: nil.
+
+Check (nil, (phi1 => phi') :: nil) :: nil .
+
+Definition Delta1 : Map Rule (Map (list Rule) (list Rule)) :=
+        (phi => phi', (nil, (phi1 => phi') :: nil) :: nil)
+     :: (phi1 => phi', (nil, (phi21 => phi') :: (phi22 => phi') :: nil) :: nil)
+     :: (phi21 => phi', (nil, (phi3 => phi') :: nil) :: nil)
+     :: (phi3 => phi', (nil, (phi4 => phi') :: nil) :: nil)
+     :: (phi4 => phi', (nil, (phi5 => phi') :: nil) :: nil)
+     :: (phi5 => phi', ((phi => phi') :: nil, (phi' => phi') :: nil) :: nil)
+     :: nil.
+
 
 Definition Valid1 : Map Formula bool :=
-  (symF (symB true), true) :: nil.
+  (impliesF phi1 phi', true) :: nil .
+Definition Valid2 : Map Formula bool :=
+  (impliesF phi5 phi', true) :: nil .
 
-Open Scope string_scope.
-Definition G :=
-  ((bp (cfg
-         ((stmtAssign "n" (aExpSymInt (symZ 2))) ~> kdot)
-         (("n", symZ 4) :: nil)
-      ))
-  =>
-  (bp (cfg
-         (kdot)
-         (("n", symZ 2) :: nil)
-      )))
-    :: nil.
 
-Eval compute in (prove 10 G G Valid1 Derivable DeltaS) .
 
+Definition ChooseCirc1 : Map Formula Rule :=
+  (phi5, phi => phi') :: nil.
+Definition ChooseCirc2 : Map Formula Rule :=
+  (phi1, phi => phi') :: nil.
+
+
+
+Print prove.
+
+
+Eval compute in (prove 10
+                       ((phi => phi') :: nil)
+                       ((phi1 => phi') :: nil)
+                       nil Valid1 Derivable1 Delta1 ChooseCirc1) .
+
+(*
+Eval compute in bGetFromMap Valid2 (impliesF phi1 phi') .
+Eval compute in Map.get Formula Rule ChooseCirc2 phi1 Formula_beq.
+Eval compute in (delta (phi => phi') ((phi => phi') :: nil) Delta1).
 *)
+
+Eval compute in (prove 10
+                       ((phi => phi') :: nil)
+                       ((phi1 => phi') :: nil)
+                       nil Valid2 Derivable1 Delta1 ChooseCirc1) .
