src/coq/procedure/Model.v
@@ -12,12 +12,15 @@ Module ImpModel .
                     | symMult : SymInt -> SymInt -> SymInt .
   Inductive SymBool := symB : bool -> SymBool
                      | symBool : string -> SymBool
+                     | symLeqInt : SymInt -> SymInt -> SymBool 
                      | symLeInt : SymInt -> SymInt -> SymBool 
                      | symEqInt : SymInt -> SymInt -> SymBool 
                      | symNeg : SymBool -> SymBool 
                      | symAnd : SymBool -> SymBool -> SymBool .
   
-
+  Scheme Equality for SymInt.
+  Scheme Equality for SymBool.
+  
     (* State *)
   Definition State := list (string * SymInt) .
 
@@ -46,5 +49,46 @@ Eval compute in (update "c" 3 (("c", 10)::("b", 5)::nil)).
 Eval compute in (update "a" 3 (("c", 10)::("b", 5)::nil)).
 Eval compute in (update "b" 3 nil).
    *)
+
+  (* S1 in S2 *)
+  Fixpoint stateIncl (S1 S2 : State) :=
+    match S1 with
+      | (k, v) :: tl => match lookup k S2 with
+                          | Some v' => if (SymInt_beq v v')
+                                       then stateIncl tl S2
+                                       else false
+                          | None => false
+                        end
+      | nil => true
+    end.
+
+  (*
+  Open Scope string_scope.
+  Eval compute in SymInt_beq (symZ 10) (symZ 10) .
+  Eval compute in stateIncl
+                    (("c", (symZ 10))::("b", (symZ 5))::nil)
+                    (("c", (symZ 10))::("b", (symZ 5))::nil) .
+  Eval compute in stateIncl
+                    (("c", (symZ 10))::("b", (symZ 5))::nil)
+                    (("c", (symZ 10))::nil) .
+  Eval compute in stateIncl
+                    (("c", (symZ 10))::nil)
+                    (("c", (symZ 10))::("b", (symZ 5))::nil) .
+   *)
   
+  Definition State_beq (S1 S2 : State) := andb (stateIncl S1 S2) (stateIncl S2 S1) .
+
+  (*
+  Open Scope string_scope.
+  Eval compute in State_beq
+                    (("c", (symZ 10))::("b", (symZ 5))::nil)
+                    (("c", (symZ 10))::("b", (symZ 5))::nil) .
+  Eval compute in State_beq
+                    (("c", (symZ 10))::("b", (symZ 5))::nil)
+                    (("c", (symZ 10))::nil) .
+  Eval compute in State_beq
+                    (("c", (symZ 10))::nil)
+                    (("c", (symZ 10))::("b", (symZ 5))::nil) .
+  Eval compute in State_beq nil nil .
+  *)
 End ImpModel .
